WIP

src/specs/PointSubAssign.ec
@@ -6,6 +6,7 @@ require import EllipticCurve.
 require import Logic.
 require import Memory.
 require import PointAddAssign.
+require import PointAddIntoDest.
 require import PointNegate.
 require import PurePrimops.
 require import Real.
@@ -40,16 +41,32 @@ module PointSubAssign = {
     }
   }
 
+  proc low'(p1, p2) = {
+    var _1, _5, _6, _9;
+    _1 <@ Primops.mload(p1);
+    Primops.mstore(W256.zero, _1);
+    _5 <@ Primops.mload(p1 + W256.of_int 32);
+    Primops.mstore(W256.of_int 32, _5);
+    _6 <@ Primops.mload(p2);
+    Primops.mstore(W256.of_int 64, _6);
+    _9 <@ Primops.mload(p2 + W256.of_int 32);
+    Primops.mstore(W256.of_int 96, _9);
+    PointNegate.low(W256.of_int 64);
+    PointAddIntoDest.low(W256.zero, W256.of_int 64, p1);
+  }
+
   proc mid(p1: int*int, p2: int*int): (int*int) option = {
-    var neg_p2, neg_p2_F, neg_p2_opt, p1_F, ret;
-    neg_p2_opt <@ PointNegate.mid(p2);
-    if (neg_p2_opt = None) {
+    var neg_p2, neg_p2_opt, ret;
+
+    if (p2.`2 = 0) {
       ret <- None;
     } else {
+      neg_p2_opt <@ PointNegate.mid(p2); (* PointNegate guaranteed to succeed here *)
       neg_p2 <- odflt (0,0) neg_p2_opt;
-      ret <@ PointAddAssign.mid(p1, neg_p2);
+      ret <@ PointAddIntoDest.mid(p1.`1, p1.`2, neg_p2.`1, neg_p2.`2);
     }
-    return (omap from_point ret);
+    
+    return ret;
   }
 }.
 
@@ -64,7 +81,65 @@ proof.
   seq 26 10: (#pre /\ ={_16}).
   inline*. wp. skip. rewrite /Constants.Q. by progress.
   inline*. wp. skip. by progress.
-qed.  
+qed.
+
+lemma pointSubAssign_low_equiv_low' :
+    equiv [
+      PointSubAssign.low ~ PointSubAssign.low':
+      ={arg, glob PointSubAssign} ==>
+      (Primops.reverted{1} /\ Primops.reverted{2}) \/
+      ={res, glob PointSubAssign}
+    ].
+    proof.
+      proc.
+      seq 7 7: (#pre /\ ={_9}). inline*. wp. skip. by progress.
+      inline PointAddIntoDest.low.
+    case (_9{1} = W256.zero).
+      seq 4 0: (Primops.reverted{1}).
+      inline Primops.mstore Primops.gas.
+      exists* p1{1}.
+      sp. elim* => memory p1.
+      seq 1 0: (_16{1} = W256.zero).
+      call{1} (
+        ConcretePrimops.staticcall_ec_add_pspec
+        (store memory (W256.of_int 96) (W256.of_int Constants.Q))
+        (load memory W256.zero, load memory (W256.of_int 32))
+        (load memory (W256.of_int 64), W256.of_int Constants.Q)
+        W256.zero
+        p1
+      ).
+          skip. progress.
+          rewrite load_store_diff. smt (@W256 @Utils). smt (@W256 @Utils). reflexivity.
+          rewrite load_store_diff. smt (@W256 @Utils). smt (@W256 @Utils). reflexivity.
+          rewrite load_store_diff. smt (@W256 @Utils). smt (@W256 @Utils). reflexivity.
+          rewrite load_store_same. reflexivity.
+      apply (weaken_and_left (result = W256.zero) (memory_L = store Primops.memory{2} (W256.of_int 96) (W256.of_int Constants.Q))).
+          apply H4. rewrite /staticcall_ec_add_should_succeed.
+          have H_malformed: !(ConcretePrimops.point_wellformed (load Primops.memory{2} (W256.of_int 64), W256.of_int Constants.Q)).
+      rewrite /point_wellformed.
+      
+
+
+    
+      seq 8 0: (load Primops.memory{1} (W256.of_int 96) = (W256.of_int Constants.Q)).
+      inline*. wp. skip. progress. rewri
+      seq 8 9: ((Primops.reverted{1} /\ Primops.reverted{2}
+      (* exists* Primops.memory{2}, p1{2}, p2{2}.
+      elim*=> memory p1 p2.
+      pose p1_x := load memory p1.
+      pose p1_y := load memory (p1 + W256.of_int 32).
+      pose p2_x := load memory p2.
+      pose p2_y := load memory (p2 + W256.of_int 32).
+      pose mem_1 := store memory W256.zero p1_x.
+      pose mem_2 := store mem_1 (W256.of_int 32) p1_y.
+      pose mem_3 := store mem_2 (W256.of_int 64) p2_x.
+      seq 7 7: (
+        Primops.memory{1} = mem_3 /\ Primops.memory{2} = mem_3 /\
+        _9{1} = p2_y /\ _9{2} = p2_y
+      ). inline*. wp. skip. progress. *)
+        seq 1 2: ((Primops.reverted{1} /\ Primops.reverted{2}) \/ ={Primops.memory}).
+      inline Primops.mstore. sp.
+      call{2} (pointNegate_low_equiv_mid Primops.memory{2} (W256.of_int 64).
 
 op pointSubAssign_memory_footprint (memory: mem) (p1: uint256): mem. (* =
   let mem_1 = store memory W256.zero (load memory p1) in
